raw_data_item_uint64_optimize_valid

src/cbor/spec/CBOR.Spec.Util.fst
@@ -1233,6 +1233,22 @@ let rec list_of_pair_list_length
 let apply_on_pair (#a #b: Type) (f: a -> b) (x: (a & a)) : Tot (b & b) =
   (f (fst x), f (snd x))
 
+let rec list_map_fst_apply_on_pair
+  (#a #b: Type) (f: a -> b) (l: list (a & a))
+: Lemma
+  (List.Tot.map fst (List.Tot.map (apply_on_pair f) l) == List.Tot.map f (List.Tot.map fst l))
+= match l with
+  | [] -> ()
+  | _ :: q -> list_map_fst_apply_on_pair f q
+
+let rec list_map_snd_apply_on_pair
+  (#a #b: Type) (f: a -> b) (l: list (a & a))
+: Lemma
+  (List.Tot.map snd (List.Tot.map (apply_on_pair f) l) == List.Tot.map f (List.Tot.map snd l))
+= match l with
+  | [] -> ()
+  | _ :: q -> list_map_snd_apply_on_pair f q
+
 let rec list_map_ext (#t #t': Type) (f1 f2: t -> t') (l: list t) (prf: (x: t { List.Tot.memP x l /\ x << l }) -> Lemma
   (f1 x == f2 x)
 ) : Lemma
@@ -1251,6 +1267,38 @@ let rec list_setoid_assoc
 = match l with
   | [] -> None
   | (a, v) :: q -> if equiv x a then Some v else list_setoid_assoc equiv x q
+
+let rec list_setoid_assoc_equiv_list
+  (#t1: Type)
+  (#t2: Type)
+  (equiv1: t1 -> t1 -> bool {
+    (forall x y . equiv1 x y == equiv1 y x) /\
+    order_trans equiv1
+  })
+  (equiv2: t2 -> t2 -> bool)
+  (l l': list (t1 & t2))
+  (x: t1)
+: Lemma
+  (requires (list_for_all2 equiv1 (List.Tot.map fst l) (List.Tot.map fst l') /\
+    list_for_all2 equiv2 (List.Tot.map snd l) (List.Tot.map snd l')
+  ))
+  (ensures (
+    match list_setoid_assoc equiv1 x l, list_setoid_assoc equiv1 x l' with
+    | None, None -> True
+    | Some y, Some y' -> equiv2 y y'
+    | _ -> False
+  ))
+  (decreases l)
+= match l with
+  | [] -> ()
+  | (a, v) :: q ->
+    let (a', v') :: q' = l' in
+    if equiv1 x a
+    then begin
+      assert (equiv1 x a');
+      assert (equiv2 v v')
+    end
+    else list_setoid_assoc_equiv_list equiv1 equiv2 q q' x
 
 let rec list_setoid_assoc_equiv_gen
   (#t1: Type)
@@ -1491,6 +1539,67 @@ let list_setoid_assoc_eq_refl
     List.Tot.for_all (setoid_assoc_eq equiv1 equiv2 l) l
   ))
 = list_setoid_assoc_eq_refl_gen equiv1 equiv2 [] l
+
+let list_setoid_assoc_eq_equiv1
+  (#t1: Type)
+  (#t2: Type)
+  (equiv1: t1 -> t1 -> bool {
+    (forall xl xr . equiv1 xl xr == equiv1 xr xl) /\
+    (forall xl xm xr . (equiv1 xl xm /\ equiv1 xm xr) ==> equiv1 xl xr)
+  })
+  (equiv2: t2 -> t2 -> bool {
+    (forall xl xr . equiv2 xl xr == equiv2 xr xl) /\
+    (forall xl xm xr . (equiv2 xl xm /\ equiv2 xm xr) ==> equiv2 xl xr)
+  })
+  (lin lin' lout: list (t1 & t2))
+: Lemma
+  (requires (
+    List.Tot.for_all (setoid_assoc_eq equiv1 equiv2 lin) lout /\
+    list_for_all2 equiv1 (List.Tot.map fst lin) (List.Tot.map fst lin') /\
+    list_for_all2 equiv2 (List.Tot.map snd lin) (List.Tot.map snd lin')
+  ))
+  (ensures (
+    List.Tot.for_all (setoid_assoc_eq equiv1 equiv2 lin') lout
+  ))
+= list_for_all_ext
+    (setoid_assoc_eq equiv1 equiv2 lin)
+    (setoid_assoc_eq equiv1 equiv2 lin')
+    lout
+    (fun x ->
+      list_setoid_assoc_equiv_list equiv1 equiv2 lin lin' (fst x);
+      ()
+    )
+
+let rec list_setoid_assoc_eq_equiv2
+  (#t1: Type)
+  (#t2: Type)
+  (equiv1: t1 -> t1 -> bool {
+    (forall x . equiv1 x x) /\
+    (forall xl xr . equiv1 xl xr == equiv1 xr xl) /\
+    (forall xl xm xr . (equiv1 xl xm /\ equiv1 xm xr) ==> equiv1 xl xr)
+  })
+  (equiv2: t2 -> t2 -> bool {
+    (forall xl xr . equiv2 xl xr == equiv2 xr xl) /\
+    (forall xl xm xr . (equiv2 xl xm /\ equiv2 xm xr) ==> equiv2 xl xr)
+  })
+  (lin lout lout': list (t1 & t2))
+: Lemma
+  (requires (
+    List.Tot.for_all (setoid_assoc_eq equiv1 equiv2 lin) lout /\
+    list_for_all2 equiv1 (List.Tot.map fst lout) (List.Tot.map fst lout') /\
+    list_for_all2 equiv2 (List.Tot.map snd lout) (List.Tot.map snd lout')
+  ))
+  (ensures (
+    List.Tot.for_all (setoid_assoc_eq equiv1 equiv2 lin) lout'
+  ))
+  (decreases lout)
+= match lout with
+  | [] -> ()
+  | (k, v) :: q ->
+    let (k', v') :: q' = lout' in
+    list_setoid_assoc_equiv equiv1 lin k k';
+    list_setoid_assoc_eq_equiv2 equiv1 equiv2 lin q q';
+    ()
 
 let list_assoc_append
     (#tk: eqtype)
